theories/lockFreeMSQ_derived.v
@@ -24,31 +24,31 @@ Variable N : namespace.
 
 (* ===== Sequential Specification for Lock-Free M&S Queue ===== *)
 
-Definition is_queue_seq (v_q : val) (xs_v: list val) (Q_γH: Qgnames) : iProp Σ :=
-  is_queue N v_q Q_γH ∗
-  Q_γH.(γ_Abst) ⤇◯ xs_v.
+Definition isQueue_S (v_q : val) (xs_v: list val) (G: Qgnames) : iProp Σ :=
+  isQueue N v_q G ∗
+  G.(γ_Abst) ⤇◯ xs_v.
 
 Lemma initialize_spec_seq :
   {{{ True }}}
     initialize #()
-  {{{ v_q Q_γH, RET v_q; is_queue_seq v_q [] Q_γH }}}.
+  {{{ v_q G, RET v_q; isQueue_S v_q [] G }}}.
 Proof.
   iIntros (Φ _) "HΦ".
   wp_apply (initialize_spec N); first done.
-  iIntros (v_q Q_γH) "[His_queue Habst_frag]".
-  iApply ("HΦ" $! v_q Q_γH).
+  iIntros (v_q G) "[HisQueue Habst_frag]".
+  iApply ("HΦ" $! v_q G).
   by iFrame.
 Qed.
 
-Lemma enqueue_spec_seq v_q (v : val) (xs_v : list val) (Q_γH : Qgnames) :
-  {{{ is_queue_seq v_q xs_v Q_γH }}}
+Lemma enqueue_spec_seq v_q (v : val) (xs_v : list val) (G : Qgnames) :
+  {{{ isQueue_S v_q xs_v G }}}
     enqueue v_q v
-  {{{w, RET w; is_queue_seq v_q (v :: xs_v) Q_γH }}}.
+  {{{w, RET w; isQueue_S v_q (v :: xs_v) G }}}.
 Proof.
-  iIntros (Φ) "(#His_queue & Hfrag) HΦ".
-  set (P := (Q_γH.(γ_Abst) ⤇◯ xs_v)%I).
-  set (Q := (Q_γH.(γ_Abst) ⤇◯ (v :: xs_v))%I).
-  wp_apply (enqueue_spec N v_q v Q_γH P Q with "[] [Hfrag]").
+  iIntros (Φ) "(#HisQueue & Hfrag) HΦ".
+  set (P := (G.(γ_Abst) ⤇◯ xs_v)%I).
+  set (Q := (G.(γ_Abst) ⤇◯ (v :: xs_v))%I).
+  wp_apply (enqueue_spec N v_q v G P Q with "[] [Hfrag]").
   (* Proving viewshift *)
   {
     iIntros (xs_v') "!>".
@@ -64,19 +64,19 @@ Proof.
   by repeat iSplit.
 Qed.
 
-Lemma dequeue_spec_seq v_q (xs_v : list val) (Q_γH : Qgnames) :
-  {{{ is_queue_seq v_q xs_v Q_γH }}}
+Lemma dequeue_spec_seq v_q (xs_v : list val) (G : Qgnames) :
+  {{{ isQueue_S v_q xs_v G }}}
     dequeue v_q
-  {{{ w, RET w; (⌜xs_v = []⌝ ∗ ⌜w = NONEV⌝ ∗ is_queue_seq v_q xs_v Q_γH) ∨
+  {{{ w, RET w; (⌜xs_v = []⌝ ∗ ⌜w = NONEV⌝ ∗ isQueue_S v_q xs_v G) ∨
                 (∃v xs_v', ⌜xs_v = xs_v' ++ [v]⌝ ∗
-                    ⌜w = SOMEV v⌝ ∗ is_queue_seq v_q xs_v' Q_γH) }}}.
+                    ⌜w = SOMEV v⌝ ∗ isQueue_S v_q xs_v' G) }}}.
 Proof.
-  iIntros (Φ) "(#His_queue & Hfrag) HΦ".
-  set (P := (Q_γH.(γ_Abst) ⤇◯ xs_v)%I).
-  set (Q := λ w, ((⌜xs_v = []⌝ ∗ ⌜w = NONEV⌝ ∗ Q_γH.(γ_Abst) ⤇◯ xs_v) ∨
+  iIntros (Φ) "(#HisQueue & Hfrag) HΦ".
+  set (P := (G.(γ_Abst) ⤇◯ xs_v)%I).
+  set (Q := λ w, ((⌜xs_v = []⌝ ∗ ⌜w = NONEV⌝ ∗ G.(γ_Abst) ⤇◯ xs_v) ∨
                   (∃v xs_v', ⌜xs_v = xs_v' ++ [v]⌝ ∗
-                    ⌜w = SOMEV v⌝ ∗ Q_γH.(γ_Abst) ⤇◯ xs_v'))%I).
-  wp_apply (dequeue_spec N v_q Q_γH P Q with "[] [Hfrag]" ).
+                    ⌜w = SOMEV v⌝ ∗ G.(γ_Abst) ⤇◯ xs_v'))%I).
+  wp_apply (dequeue_spec N v_q G P Q with "[] [Hfrag]" ).
   (* Proving viewshift *)
   {
     iIntros (xs_v') "!>".
@@ -127,37 +127,37 @@ Notation NC := (N .@ "concurrent").
 
 (* ===== Concurrent Specification for Lock-Free M&S Queue ===== *)
 
-Definition is_queue_conc (Ψ : val -> iProp Σ) (v_q : val) (Q_γH: Qgnames) : iProp Σ :=
-  is_queue N v_q Q_γH ∗
-  inv NC (∃xs_v, Q_γH.(γ_Abst) ⤇◯ xs_v ∗ All xs_v Ψ).
+Definition isQueue_C (Ψ : val -> iProp Σ) (v_q : val) (G: Qgnames) : iProp Σ :=
+  isQueue N v_q G ∗
+  inv NC (∃xs_v, G.(γ_Abst) ⤇◯ xs_v ∗ All xs_v Ψ).
 
-(* is_queue_conc is persistent *)
-Global Instance is_queue_conc_persistent Ψ v_q Q_γH : Persistent (is_queue_conc Ψ v_q Q_γH).
+(* isQueue_C is persistent *)
+Global Instance isQueue_C_persistent Ψ v_q G : Persistent (isQueue_C Ψ v_q G).
 Proof. apply _. Qed.
 
 Lemma initialize_spec_conc (Ψ : val -> iProp Σ):
   {{{ True }}}
     initialize #()
-  {{{ v_q Q_γH, RET v_q; is_queue_conc Ψ v_q Q_γH }}}.
+  {{{ v_q G, RET v_q; isQueue_C Ψ v_q G }}}.
 Proof.
   iIntros (Φ _) "HΦ".
   iApply wp_fupd.
   wp_apply (initialize_spec N); first done.
-  iIntros (v_q Q_γH) "[His_queue Habst_frag]".
-  iApply ("HΦ" $! v_q Q_γH).
-  iMod (inv_alloc NC _ (∃xs_v, Q_γH.(γ_Abst) ⤇◯ xs_v ∗ All xs_v Ψ) with "[Habst_frag]") as "HInv"; first (iExists []; auto).
+  iIntros (v_q G) "[HisQueue Habst_frag]".
+  iApply ("HΦ" $! v_q G).
+  iMod (inv_alloc NC _ (∃xs_v, G.(γ_Abst) ⤇◯ xs_v ∗ All xs_v Ψ) with "[Habst_frag]") as "HInv"; first (iExists []; auto).
   by iFrame.
 Qed.
 
-Lemma enqueue_spec_conc v_q Ψ (v : val) (Q_γH : Qgnames) :
-  {{{ is_queue_conc Ψ v_q Q_γH ∗ Ψ v }}}
+Lemma enqueue_spec_conc v_q Ψ (v : val) (G : Qgnames) :
+  {{{ isQueue_C Ψ v_q G ∗ Ψ v }}}
     enqueue v_q v
   {{{ w, RET w; True }}}.
 Proof.
-  iIntros (Φ) "[(#His_queue & #HInv) HΨ] HΦ".
+  iIntros (Φ) "[(#HisQueue & #HInv) HΨ] HΦ".
   set (P := Ψ v).
   set (Q := True%I).
-  wp_apply (enqueue_spec N v_q v Q_γH P Q with "[] [HΨ]").
+  wp_apply (enqueue_spec N v_q v G P Q with "[] [HΨ]").
   (* Proving viewshift *)
   {
     iIntros (xs_v') "!>".
@@ -179,15 +179,15 @@ Proof.
   by iApply ("HΦ" $! w).
 Qed.
 
-Lemma dequeue_spec_conc v_q Ψ (Q_γH : Qgnames) :
-  {{{ is_queue_conc Ψ v_q Q_γH }}}
+Lemma dequeue_spec_conc v_q Ψ (G : Qgnames) :
+  {{{ isQueue_C Ψ v_q G }}}
     dequeue v_q
   {{{ w, RET w; ⌜w = NONEV⌝ ∨ (∃ v, ⌜w = SOMEV v⌝ ∗ Ψ v) }}}.
 Proof.
-  iIntros (Φ) "(#His_queue & #HInv) HΦ".
+  iIntros (Φ) "(#HisQueue & #HInv) HΦ".
   set (P := True%I : iProp Σ).
   set (Q := λ w, (⌜w = NONEV⌝ ∨ (∃v, ⌜w = SOMEV v⌝ ∗ Ψ v))%I).
-  wp_apply (dequeue_spec N v_q Q_γH P Q).
+  wp_apply (dequeue_spec N v_q G P Q).
   (* Proving viewshift *)
   {
     iIntros (xs_v') "!>".
