Tasks.md
@@ -111,17 +111,12 @@
 - [x] change null / null node / ... to None
 - [x] Consider not using the term "sentinel"
 - [x] change "x" to ``x'', and similarly for 'x'
-- [ ] Decide on name/notation for Qgnames (including SeqQgnames and ConcQgnames). Maybe \mathcal(G)_{\text{seq}}?
 - [x] Center figures on page (not on line)
 - [x] Make sure all node values are 'w' and queue values are 'v'
 - [x] Rewrite some of the proofs for two-lock
 - [x] Consider adding the specifications for the derivation proofs
 - [x] Refer to line numbers in proofs for two-lock
 - [ ] Check for correctness of line number references
-- [ ] Format the forall intros in lemmas (and definitions) better
-- [ ] Change is_queue to isQueue
-- [ ] Change is_queue_seq to isQueue_{seq} and similarly for conc
-- [ ] Use camelCase for predicates. (proj_val, wrap_some, proj_gnames...)
 - [x] Proofread sequential and concurrent derivation section
 - [x] refactor specification macros to take the forall quantified variables as input
 - [x] Also make hocap viewshifts their own macros
@@ -141,25 +136,33 @@
   - [x] Iris Lecture Notes (see todos in report)
   - [x] Herlihy & Wing : Linearizability. #5 in MSQ paper
 
-- [ ] If time permits, use hocap spec to prove a spec of a client
-- [ ] change cite to citet or citep
+
+- [ ] Decide on name/notation for Qgnames (including SeqQgnames and ConcQgnames). Maybe \mathcal(G)_{\text{seq}}?
+- [ ] Format the forall intros in lemmas (and definitions) better
+- [x] Change is_queue to isQueue
+- [x] Change is_queue_seq to isQueue_{seq} and similarly for conc
+- [x] Use camelCase for predicates. (proj_val, wrap_some, proj_gnames...)
+- [x] change cite to citet or citep
 - [ ] Always start sentences with capital letter. Change sentences that start with variables to enforce this
 - [ ] only use "points to" for predicate
 - [ ] don't use future tense so much
-- [ ] Another way to mark persistent pointers in figures
+- [x] Use another way to mark persistent pointers in figures (maybe a square above or on it)
 - [ ] Consider moving observations to the enqueue and dequeue functions. some inside sections and others after
-- [ ] Make line numbers continuous across functions. init start at 1, enq start at where init ended...
-- [ ] For figures, explain the assumption that the head doesn't change during the enqueue (no dequeue happens) (possibly in the figure text)
-- [ ] Change Q_γ to G in coq
-- [ ] add {} before \star and any other binary operators
+- [x] Make line numbers continuous across functions. init start at 1, enq start at where init ended...
+- [x] For figures, explain the assumption that the head doesn't change during the enqueue (no dequeue happens) (possibly in the figure text)
+- [x] Change Q_γ to G in coq
+- [x] add {} before \star and any other binary operators
 - [ ] move Resource Algebra specifics into chapter on resource algebra
   - [ ] Definition of RA's, e.g. Ex()
   - [ ] Show useful lemmas about the RA's in the sections where they are used
-- [ ] Change ToknE to TokNE. similarly for rest
-  - [ ] Tok_{NE}
-  - [ ] also change in coq
+- [x] Change ToknE to TokNE. similarly for rest
+  - [x] also change in coq
 - [ ] move definition of simpler concurrent queue invariant out of appendix, into report
 - [ ] Move definitions of hocap invariant and queue predicate out of appendix, into section
 - [ ] do not use contractions
-- [ ] Change "spec" to "specification"
+- [x] Change "spec" to "specification"
+- [ ] Consider removing 'tl' and 'lf' prefixes for latex macros for specifications
+- [ ] Rewrite moved sections and chapters to get a red line again
 - [ ] Check if any extra todos from Amin's feedback
+
+- [ ] If time permits, use hocap spec to prove a spec of a client
